More progress on mix columns

nat_to_byte_gen.py
@@ -20,3 +20,23 @@ function += "\n  end."
 
 print(function)
 
+
+function = """
+Definition byte_to_nat(a : byte) : nat := 
+match a with \n"""
+
+
+for i in range(256):
+  s = "{0:b}".format(i)
+  sr = ""
+  for j in range(8-len(s)):
+    sr += "s0 "
+  for j in range(len(s)):
+    sr += "s"+s[j]+" "
+  function += "| bits8 "+sr+" => "+str(i)+" \n"
+
+
+function += "\n  end."
+
+
+print(function)
